String-based SMTLIB, drop name bijection

bin/driver/SMTPP.ml
@@ -6,15 +6,11 @@ module SMTLib = struct
     | Sort_BitVec n -> fprintf fmt "(_ BitVec %a)" Z.pp_print n
     | _ -> failwith "Unexpected sort"
 
-  let varName (nameMap : VerilogSMTBijection.t) fmt nameIdx =
-    match nameMap.bij_inverse nameIdx with
-    | Some (VerilogLeft, n) -> fprintf fmt "|l_%s|" (Util.lst_to_string n.varName)
-    | Some (VerilogRight, n) ->
-        fprintf fmt "|r_%s|" (Util.lst_to_string n.varName)
-    | None -> fprintf fmt "|v%a|" Z.pp_print (int_from_nat nameIdx)
+  let varName fmt smtname =
+    fprintf fmt "|%s|" smtname
 
-  let var (nameMap : VerilogSMTBijection.t) fmt ((nameIdx, s) : smtname * sort) =
-    fprintf fmt "(as %a %a)" (varName nameMap) nameIdx sort s 
+  let var fmt (sym : const_sym) =
+    fprintf fmt "(as %a %a)" varName sym.symName sort sym.symSort 
 
   let bitvector fmt (bits : bool list) =
     fprintf fmt "#b%s"
@@ -35,84 +31,81 @@ module SMTLib = struct
     | BVShl -> fprintf fmt "bvshl"
     | BVShr -> fprintf fmt "bvlshr"
 
-  let rec term varNames fmt = function
-    | Term_Const (s, name) -> var varNames fmt (name, s)
+  let rec term fmt = function
+    | Term_Const sym -> var fmt sym
     | Term_Eq (_s, l, r) ->
-        fprintf fmt "(= %a %a)" (term varNames) l (term varNames) r
+        fprintf fmt "(= %a %a)" term l term r
     | Term_And (l, r) ->
-        fprintf fmt "(and %a %a)" (term varNames) l (term varNames) r
+        fprintf fmt "(and %a %a)" term l term r
     | Term_Or (l, r) ->
-        fprintf fmt "(or %a %a)" (term varNames) l (term varNames) r
-    | Term_Not t -> fprintf fmt "(not %a)" (term varNames) t
+        fprintf fmt "(or %a %a)" term l term r
+    | Term_Not t -> fprintf fmt "(not %a)" term t
     | Term_ITE (_s, t1, t2, t3) ->
-        fprintf fmt "(ite %a %a %a)" (term varNames) t1 (term varNames) t2
-          (term varNames) t3
+        fprintf fmt "(ite %a %a %a)" term t1 term t2
+          term t3
     | Term_True -> fprintf fmt "true"
     | Term_False -> fprintf fmt "false"
     | Term_BVLit (_, bv) -> bitvector fmt bv
     | Term_BVConcat (_, _, l, r) ->
-        fprintf fmt "(concat %a %a)" (term varNames) l (term varNames) r
+        fprintf fmt "(concat %a %a)" term l term r
     | Term_BVExtract (_, lo, hi, t) ->
         fprintf fmt "((_ extract %a %a) %a)" Z.pp_print (int_from_nat lo)
-          Z.pp_print (int_from_nat hi) (term varNames) t
+          Z.pp_print (int_from_nat hi) term t
     | Term_BVUnaryOp (_, op, t) ->
-        fprintf fmt "(%a %a)" unaryOp op (term varNames) t
+        fprintf fmt "(%a %a)" unaryOp op term t
     | Term_BVBinOp (_, op, t1, t2) ->
-        fprintf fmt "(%a %a %a)" binaryOp op (term varNames) t1 (term varNames)
+        fprintf fmt "(%a %a %a)" binaryOp op term t1 term
           t2
     | Term_BVUlt (_, t1, t2) ->
-        fprintf fmt "(bvult %a %a)" (term varNames) t1 (term varNames) t2
+        fprintf fmt "(bvult %a %a)" term t1 term t2
 
-  module SMTNameMap = struct
-    include Map.Make(struct type t = smtname let compare = compare end)
-    let combine = union (fun _ s _ -> Some s)
-  end
+  module SMTVarSet = Set.Make(struct type t = const_sym let compare = compare end)
 
-  let rec collect_declarations_term : term -> sort SMTNameMap.t = function
-    | Term_Const (s, name) -> SMTNameMap.singleton name s
+  let rec collect_declarations_term : term -> SMTVarSet.t = function
+    | Term_Const sym -> SMTVarSet.singleton sym
     | Term_Eq (_s, l, r) ->
-        SMTNameMap.combine (collect_declarations_term l) (collect_declarations_term r)
+        SMTVarSet.union (collect_declarations_term l) (collect_declarations_term r)
     | Term_And (l, r) ->
-        SMTNameMap.combine (collect_declarations_term l) (collect_declarations_term r)
+        SMTVarSet.union (collect_declarations_term l) (collect_declarations_term r)
     | Term_Or (l, r) ->
-        SMTNameMap.combine (collect_declarations_term l) (collect_declarations_term r)
+        SMTVarSet.union (collect_declarations_term l) (collect_declarations_term r)
     | Term_Not t -> collect_declarations_term t
     | Term_ITE (_s, t1, t2, t3) ->
-        SMTNameMap.combine
-          (SMTNameMap.combine (collect_declarations_term t1) (collect_declarations_term t2))
+        SMTVarSet.union
+          (SMTVarSet.union (collect_declarations_term t1) (collect_declarations_term t2))
           (collect_declarations_term t3)
-    | Term_True -> SMTNameMap.empty
-    | Term_False -> SMTNameMap.empty
-    | Term_BVLit (_, _bv) -> SMTNameMap.empty
+    | Term_True -> SMTVarSet.empty
+    | Term_False -> SMTVarSet.empty
+    | Term_BVLit (_, _bv) -> SMTVarSet.empty
     | Term_BVConcat (_, _, l, r) ->
-        SMTNameMap.combine (collect_declarations_term l) (collect_declarations_term r)
+        SMTVarSet.union (collect_declarations_term l) (collect_declarations_term r)
     | Term_BVExtract (_, _lo, _hi, t) -> collect_declarations_term t
     | Term_BVUnaryOp (_, _, t) -> collect_declarations_term t
     | Term_BVBinOp (_, _op, t1, t2) ->
-        SMTNameMap.combine (collect_declarations_term t1) (collect_declarations_term t2)
+        SMTVarSet.union (collect_declarations_term t1) (collect_declarations_term t2)
     | Term_BVUlt (_, t1, t2) ->
-        SMTNameMap.combine (collect_declarations_term t1) (collect_declarations_term t2)
+        SMTVarSet.union (collect_declarations_term t1) (collect_declarations_term t2)
 
-  let collect_declarations : query -> sort SMTNameMap.t =
-    List.fold_left (fun acc t -> SMTNameMap.combine acc (collect_declarations_term t)) SMTNameMap.empty
+  let collect_declarations : query -> SMTVarSet.t =
+    List.fold_left (fun acc t -> SMTVarSet.union acc (collect_declarations_term t)) SMTVarSet.empty
 
-  let declaration nameMap fmt (v, s) =
-    fprintf fmt "(declare-const %a %a)" (varName nameMap) v sort s
+  let declaration fmt sym =
+    fprintf fmt "(declare-const %a %a)" varName sym.symName sort sym.symSort
 
-  let assertion varNames fmt t = fprintf fmt "(assert %a)" (term varNames) t
+  let assertion fmt t = fprintf fmt "(assert %a)" term t
 
-  let raw_query fmt (query : smt_with_namemap) =
+  let raw_query fmt (query : query) =
     pp_print_list
-      (declaration query.nameMap)
+      declaration
       fmt
-      (collect_declarations query.assertions |> SMTNameMap.to_seq |> List.of_seq)
+      (collect_declarations query |> SMTVarSet.to_seq |> List.of_seq)
       ~pp_sep:pp_force_newline;
     pp_force_newline fmt ();
     pp_force_newline fmt ();
-    pp_print_list (assertion query.nameMap) fmt query.assertions
+    pp_print_list assertion fmt query
       ~pp_sep:pp_force_newline
 
-  let query fmt (query : smt_with_namemap) =
+  let query fmt (query : query) =
     fprintf fmt "(set-info :smt-lib-version 2.6)\n";
     fprintf fmt "(set-logic QF_BV)\n";
     raw_query fmt query;
