vera/VerilogEquivalence.v
@@ -3,8 +3,6 @@ From vera Require VerilogSemantics.
 Import VerilogSemantics.Sort.
 From vera Require Import VerilogSMT.
 From vera Require Import Common.
-Import (coercions) VerilogSMTBijection.
-Import VerilogSMTBijection (bij_inverse, bij_apply, bij_wf).
 From vera Require AssignmentForwarding.
 From vera Require VerilogToSMT.
 From vera Require SMTQueries.
@@ -41,137 +39,26 @@ Import FunctorNotation.
 Local Open Scope monad_scope.
 Local Open Scope string.
 
-Equations mk_var_same (var : Verilog.variable) (m : VerilogSMTBijection.t)
-  : sum string (SMTLib.term SMTLib.Sort_Bool) := {
-  | var, m with m (TaggedVariable.VerilogLeft, var), m (TaggedVariable.VerilogRight, var) => {
-    | Some smt_name1, Some smt_name2 =>
-      let t := SMTLib.Sort_BitVec (Verilog.varType var)
-      in inr (SMTLib.Term_Eq (SMTLib.Term_Const t smt_name1) (SMTLib.Term_Const t smt_name2))
-    | _, _ => inl "mk_var_same"%string
-    }
-  }
+Definition mk_var_same (var : Verilog.variable) : (SMTLib.term SMTLib.Sort_Bool) := 
+  SMTLib.Term_Eq (SMTLib.Term_Const (verilog_to_smt_var VerilogLeft var))
+                 (SMTLib.Term_Const (verilog_to_smt_var VerilogRight var)).
+
+Equations mk_inputs_same (inputs : list Verilog.variable) : SMTLib.term SMTLib.Sort_Bool := {
+  | [] => SMTLib.Term_True
+  | (var :: vars) => SMTLib.Term_And (mk_var_same var) (mk_inputs_same vars)
+}.
+
+Definition mk_var_distinct (var : Verilog.variable) : SMTLib.term SMTLib.Sort_Bool :=
+  SMTLib.Term_Not (SMTLib.Term_Eq (SMTLib.Term_Const (verilog_to_smt_var VerilogLeft var))
+                                  (SMTLib.Term_Const (verilog_to_smt_var VerilogRight var)))
   .
 
-Equations mk_inputs_same (inputs : list Verilog.variable) (m : VerilogSMTBijection.t)
-  : sum string (SMTLib.term SMTLib.Sort_Bool) := {
-  | [], m => inr SMTLib.Term_True
-  | (var :: vars), m =>
-      match
-        mk_var_same var m,
-        mk_inputs_same vars m
-      with
-      | inr hd, inr tl =>
-          inr (SMTLib.Term_And hd tl)
-      | _, _ => inl "err"%string
-      end
-  }.
+Equations mk_outputs_distinct (inputs : list Verilog.variable) : SMTLib.term SMTLib.Sort_Bool := {
+  | [] => SMTLib.Term_False
+  | (var :: vars) => SMTLib.Term_Or (mk_var_distinct var) (mk_outputs_distinct vars)
+}.
 
-Equations mk_var_distinct (var : Verilog.variable) (m : VerilogSMTBijection.t)
-  : sum string (SMTLib.term SMTLib.Sort_Bool) := {
-  | var, m with m (TaggedVariable.VerilogLeft, var), m (TaggedVariable.VerilogRight, var) => {
-    | Some smt_name1, Some smt_name2 =>
-      let t := SMTLib.Sort_BitVec (Verilog.varType var)
-      in inr (SMTLib.Term_Not (SMTLib.Term_Eq (SMTLib.Term_Const t smt_name1) (SMTLib.Term_Const t smt_name2)))
-    | _, _ => inl "mk_var_distinct"%string
-    }
-  }
-  .
-
-Equations mk_outputs_distinct (inputs : list Verilog.variable) (m : VerilogSMTBijection.t)
-  : sum string (SMTLib.term SMTLib.Sort_Bool) := {
-  | [], m => inr SMTLib.Term_False
-  | (var :: vars), m =>
-      match
-        mk_var_distinct var m,
-        mk_outputs_distinct vars m
-      with
-      | inr hd, inr tl =>
-          inr (SMTLib.Term_Or hd tl)
-      | _, _ => inl "err"%string
-      end
-  }.
-
-Lemma mk_bijection_only_tag tag vars m :
-  VerilogToSMT.mk_bijection tag vars = inr m ->
-  VerilogSMTBijection.only_tag tag m.
-Proof.
-  revert m.
-  funelim (VerilogToSMT.mk_bijection tag vars); intros.
-  - inv H. apply VerilogSMTBijection.only_tag_empty.
-  - simp mk_bijection in H0; inv H0; autodestruct.
-    eauto using VerilogSMTBijection.only_tag_insert.
-Qed.
-
-Lemma verilog_to_smt_only_tag tag start v s :
-  VerilogToSMT.verilog_to_smt tag start v = inr s ->
-  VerilogSMTBijection.only_tag tag (nameMap s).
-Proof.
-  intros.
-  unfold VerilogToSMT.verilog_to_smt in *. simpl in *.
-  autodestruct_eqn E. cbn.
-  eauto using mk_bijection_only_tag.
-Qed.
-
-Lemma mk_bijection_min_name tag start vars m var name :
-  VerilogToSMT.mk_bijection tag (VerilogToSMT.assign_vars start vars) = inr m ->
-  m (tag, var) = Some name ->
-  name >= start.
-Proof.
-  revert m start.
-  induction vars; intros * Hfunc Hm; simp assign_vars mk_bijection in *.
-  - inv Hfunc. discriminate.
-  - monad_inv.
-    destruct (dec (a = var)).
-    + subst a.
-      rewrite VerilogSMTBijection.lookup_insert_in in Hm. inv Hm.
-      lia.
-    + rewrite VerilogSMTBijection.lookup_insert_out in Hm by crush.
-      insterU IHvars.
-      crush.
-Qed.
-
-Lemma verilog_to_smt_min_name tag start v s var name :
-  VerilogToSMT.verilog_to_smt tag start v = inr s ->
-  nameMap s (tag, var) = Some name ->
-  name >= start.
-Proof.
-  intros.
-  unfold VerilogToSMT.verilog_to_smt in *. simpl in *.
-  autodestruct_eqn E. simpl in *.
-  eauto using mk_bijection_min_name.
-Qed.
-
-Lemma mk_bijection_max_name vars : forall tag start m var name,
-  VerilogToSMT.mk_bijection tag (VerilogToSMT.assign_vars start vars) = inr m ->
-  m (tag, var) = Some name ->
-  name <= start + length vars.
-Proof.
-  induction vars;
-    intros * Hfunc Hm;
-    simp assign_vars mk_bijection in *; simpl in *;
-    monad_inv.
-  - discriminate.
-  - destruct (dec (a = var)).
-    + subst a.
-      rewrite VerilogSMTBijection.lookup_insert_in in Hm. inv Hm.
-      lia.
-    + rewrite VerilogSMTBijection.lookup_insert_out in Hm by crush.
-      insterU IHvars.
-      crush.
-Qed.
-
-Lemma verilog_to_smt_max_name tag start s v var name :
-  VerilogToSMT.verilog_to_smt tag start v = inr s ->
-  nameMap s (tag, var) = Some name ->
-  name <= start + length (Verilog.modVariables v).
-Proof.
-  intros Hfunc Hm.
-  unfold VerilogToSMT.verilog_to_smt in Hfunc.
-  monad_inv.
-  eapply mk_bijection_max_name; eassumption.
-Qed.
-
-Program Definition equivalence_query (verilog1 verilog2 : Verilog.vmodule) : sum string smt_with_namemap :=
+Program Definition equivalence_query (verilog1 verilog2 : Verilog.vmodule) : sum string SMTQueries.query :=
   let* inputs_ok1 :=
     assert_dec
       (Verilog.module_inputs verilog1 = Verilog.module_inputs verilog2)
@@ -187,49 +74,11 @@ Program Definition equivalence_query (verilog1 verilog2 : Verilog.vmodule) : sum
       ++ to_string (Verilog.module_outputs verilog2) )
     in
 
-  let* ( smt1 ; prf1 ) := sum_with_eqn (VerilogToSMT.verilog_to_smt TaggedVariable.VerilogLeft 0 verilog1) in
-  let* ( smt2 ; prf2 ) := sum_with_eqn (VerilogToSMT.verilog_to_smt TaggedVariable.VerilogRight (S (length (Verilog.modVariables verilog1))) verilog2) in
+  let* smt1 := VerilogToSMT.verilog_to_smt VerilogLeft verilog1 in
+  let* smt2 := VerilogToSMT.verilog_to_smt VerilogRight verilog2 in
 
-  let nameMap := VerilogSMTBijection.combine (nameMap smt1) (nameMap smt2) _ _ in
+  let inputs_same := mk_inputs_same (Verilog.module_inputs verilog1) in
+  let outputs_distinct := mk_outputs_distinct (Verilog.module_outputs verilog1) in
 
-  let* inputs_same := mk_inputs_same (Verilog.module_inputs verilog1) nameMap in
-  let* outputs_distinct := mk_outputs_distinct (Verilog.module_outputs verilog1) nameMap in
-
-  ret {|
-      nameMap := nameMap ;
-      assertions := inputs_same :: outputs_distinct :: (assertions smt1 ++ assertions smt2)
-    |}
+  inr (inputs_same :: outputs_distinct :: (smt1 ++ smt2))
 .
-Next Obligation.
-  (* No shared verilog names *)
-  repeat apply_somewhere verilog_to_smt_only_tag.
-  unfold VerilogSMTBijection.only_tag in *.
-  match goal with
-  [ |- ?x = None ] => destruct x eqn:E; [|reflexivity]
-  end.
-  rewrite VerilogSMTBijection.bij_wf in H, E.
-  apply (f_equal (option_map fst)) in H, E.
-  insterU X. insterU X0.
-  crush.
-Qed.
-Next Obligation.
-  (* No shared smt names *)
-  match goal with
-  [ |- ?x = None ] => destruct x as [[t' v']|] eqn:E; [|reflexivity]
-  end.
-  replace t with TaggedVariable.VerilogLeft in *; cycle 1. {
-    symmetry.
-    eapply verilog_to_smt_only_tag. eassumption.
-    rewrite H. reflexivity.
-  }
-  replace t' with TaggedVariable.VerilogRight in *; cycle 1. {
-    symmetry.
-    eapply verilog_to_smt_only_tag. eassumption.
-    rewrite E. reflexivity.
-  }
-  rewrite <- VerilogSMTBijection.bij_wf in H, E.
-  pose proof (verilog_to_smt_min_name TaggedVariable.VerilogLeft) as Hmin_left. insterU Hmin_left.
-  pose proof (verilog_to_smt_min_name TaggedVariable.VerilogRight) as Hmin_right. insterU Hmin_right.
-  pose proof (verilog_to_smt_max_name TaggedVariable.VerilogLeft) as Hmax_left. insterU Hmax_left.
-  lia.
-Qed.
