vera/VerilogSMT.v
@@ -1,5 +1,6 @@
 From Stdlib Require Import ZArith.
 From Stdlib Require Import BinNums.
+From Stdlib Require Import Ascii.
 From Stdlib Require Import String.
 From Stdlib Require Import List.
 From Stdlib Require Import Logic.FunctionalExtensionality.
@@ -8,6 +9,9 @@ From Stdlib Require Import Structures.Equalities.
 From Stdlib Require Import Morphisms.
 
 From Equations Require Import Equations.
+From Equations.Prop Require Import Logic.
+From ExtLib Require Import Data.Monads.EitherMonad.
+From ExtLib Require Import Structures.Monad.
 
 From vera Require Import Common.
 From vera Require Import Decidable.
@@ -24,225 +28,210 @@ Import BITVECTOR_LIST.
 From vera Require SMTLib.
 
 Import ListNotations.
-Local Open Scope list.
-
 Import SigTNotations.
+Import MonadLetNotation.
 
-Module TaggedVariable.
-  Inductive Tag :=
-  | VerilogLeft
-  | VerilogRight
-  .
+Local Open Scope list.
+Local Open Scope monad_scope.
 
-  #[global] Instance dec_eq_tag (a b : Tag) : DecProp (a = b) :=
-    mk_dec_eq.
+Inductive VarTag := VerilogLeft | VerilogRight.
 
-  Definition t := (Tag * Verilog.variable)%type.
+Definition tag_choose {A} t (x1 x2 : A) : A :=
+  match t with
+  | VerilogLeft => x1
+  | VerilogRight => x2
+  end.
 
-  Definition eq (l r : t) := l = r.
-
-  Definition eq_equiv : Equivalence eq := eq_equivalence.
-
-  Definition eq_dec (x y : t) : { eq x y } + { ~ eq x y } :=
-    dec (x = y).
-End TaggedVariable.
-
-Module VerilogSMTBijection.
-  Include PartialBijection(TaggedVariable)(NatAsUDT).
-
-  Definition only_tag t m := forall tag smtName,
-      option_map fst (bij_inverse m smtName) = Some tag ->
-      tag = t.
-
-  Lemma only_tag_empty t : only_tag t empty.
-  Proof. cbv. discriminate. Qed.
-
-  Lemma only_tag_insert tag name b m :
-    only_tag tag m ->
-    forall H1 H2,
-      only_tag tag (insert (tag, name) b m H1 H2).
-  Proof.
-    unfold insert, only_tag.
-    intros.
-    unfold option_map in *.
-    repeat (autodestruct_eqn E; cbn in * ); try reflexivity.
-    eapply H. now erewrite E.
-  Qed.
-
-  Lemma combine_different_tag_left (m1 m2 : t) (t1 t2 : TaggedVariable.Tag) prf1 prf2:
-    (t1 <> t2) ->
-    only_tag t1 m1 ->
-    only_tag t2 m2 ->
-    forall n, combine m1 m2 prf1 prf2 (t1, n) = m1 (t1, n).
-  Proof.
-    intros.
-    unfold combine. simpl.
-    destruct (m1 (t1, n)) eqn:E1; try reflexivity.
-    destruct (m2 (t1, n)) eqn:E2; try reflexivity.
-    exfalso.
-    apply bij_wf in E2.
-    erewrite (H1 t1) in H. contradiction.
-    now erewrite E2.
-  Qed.
-
-  Lemma combine_different_tag_right (m1 m2 : VerilogSMTBijection.t) (t1 t2 : TaggedVariable.Tag) prf1 prf2:
-    (t1 <> t2) ->
-    only_tag t1 m1 ->
-    only_tag t2 m2 ->
-    forall n, VerilogSMTBijection.combine m1 m2 prf1 prf2 (t2, n) = m2 (t2, n).
-  Proof.
-    intros.
-    unfold VerilogSMTBijection.combine. simpl.
-    destruct (m1 (t2, n)) eqn:E1; try reflexivity.
-    destruct (m2 (t2, n)) eqn:E2; try reflexivity.
-    - exfalso.
-      apply VerilogSMTBijection.bij_wf in E1.
-      erewrite (H0 t2) in H. contradiction.
-      now erewrite E1.
-    - exfalso.
-      apply VerilogSMTBijection.bij_wf in E1.
-      erewrite (H0 t2) in H. contradiction.
-      now erewrite E1.
-  Qed.
-End VerilogSMTBijection.
-
-Import VerilogSMTBijection (bij_inverse, bij_apply, bij_wf).
-Import (coercions) VerilogSMTBijection.
-
-Definition match_map_vars (tag : TaggedVariable.Tag) (map : VerilogSMTBijection.t) vars :=
-  forall var, (exists smtName, map (tag, var) = Some smtName) <-> (In var vars).
-
-Record smt_with_namemap :=
-  MkSMTWithNameMap
-    { assertions : SMTQueries.query;
-      nameMap : VerilogSMTBijection.t;
-    }.
-
-Definition max_declaration (q : SMTQueries.query) : nat :=
-  List.list_max (SMTQueries.domain q).
-
-Lemma max_declaration_domain q name :
-  In name (SMTQueries.domain q) ->
-  name <= max_declaration q.
-Proof.
-  unfold max_declaration, SMTQueries.domain.
-  revert name. rewrite <- Forall_forall.
-  apply list_max_le.
-  trivial.
-Qed.
+#[global] Instance dec_eq_tag (a b : VarTag) : DecProp (a = b) :=
+  mk_dec_eq.
 
 Equations default (s : SMTLib.sort) : SMTLib.interp_sort s :=
   default (SMTLib.Sort_Bool) := false;
   default (SMTLib.Sort_BitVec n) := BV.zeros n.
 
+Definition tag_name (t : VarTag) (s : string) : string :=
+  (match t with
+   | VerilogLeft => "l"
+   | VerilogRight => "r"
+   end ++ "__" ++ s)%string.
+
+Definition untag_name (s : string) : option (VarTag * string) :=
+  match s with
+  | (String "l" (String "_" (String "_" s'))) => Some (VerilogLeft, s')
+  | (String "r" (String "_" (String "_" s'))) => Some (VerilogRight, s')
+  | _ => None
+  end.
+
+Lemma tag_name_injective_tag t t' n n' :
+  tag_name t n = tag_name t' n' ->
+  t = t'.
+Proof.
+  unfold untag_name, tag_name.
+  destruct t, t'.
+  all: crush.
+Qed.
+
+Lemma tag_name_injective_name t t' n n' :
+  tag_name t n = tag_name t' n' ->
+  n = n'.
+Proof.
+  unfold untag_name, tag_name.
+  destruct t, t'.
+  all: crush.
+Qed.
+
+Lemma untag_tag_name t s : untag_name (tag_name t s) = Some (t, s).
+Proof.
+  unfold untag_name, tag_name.
+  destruct t; reflexivity.
+Qed.
+
+Lemma tag_untag_name t n n' :
+  untag_name n = Some (t, n') ->
+  tag_name t n' = n.
+Proof.
+ unfold untag_name, tag_name.
+ intros H.
+ autodestruct; reflexivity.
+Qed.
+
+Lemma tag_untag_name_none t n n' :
+  untag_name n = None ->
+  tag_name t n' <> n.
+Proof.
+ intros H contra.
+ apply f_equal with (f:=untag_name) in contra.
+ rewrite H in contra.
+ rewrite untag_tag_name in contra.
+ discriminate.
+Qed.
+
+Definition verilog_to_smt_var (t : VarTag) (var : Verilog.variable) : SMTLib.const_sym :=
+  {|
+    SMTLib.symName := tag_name t (Verilog.varName var);
+    SMTLib.symSort := SMTLib.Sort_BitVec (Verilog.varType var)
+  |}.
+
+Definition smt_to_verilog_var (sym : SMTLib.const_sym) : option (VarTag * Verilog.variable)  :=
+  let* (t, name) := untag_name (SMTLib.symName sym) in
+  let* w := match SMTLib.symSort sym with
+            | SMTLib.Sort_BitVec w => Some w
+	    | _ => None
+	    end in
+  let* prf := opt_dec (w > 0)%N in
+  Some (t, Verilog.MkVariable name w prf).
+
+Lemma verilog_to_smt_to_verilog_var t var : smt_to_verilog_var (verilog_to_smt_var t var) = Some (t, var).
+Proof.
+  unfold smt_to_verilog_var, verilog_to_smt_var.
+  destruct var.
+  simpl. rewrite untag_tag_name. monad_inv.
+  - do 3 f_equal. apply proof_irrelevance.
+  - exfalso. destruct varType; crush.
+Qed.
+
+Lemma smt_to_verilog_to_smt_var_some sym t var :
+  smt_to_verilog_var sym = Some (t, var) ->
+  verilog_to_smt_var t var = sym.
+Proof.
+  unfold smt_to_verilog_var, verilog_to_smt_var.
+  destruct sym, var.
+  intros H. monad_inv. simpl in *.
+  apply tag_untag_name in E.
+  rewrite E.
+  reflexivity.
+Qed.
+
+Lemma smt_to_verilog_to_smt_var_none sym t var :
+  smt_to_verilog_var sym = None ->
+  verilog_to_smt_var t var <> sym.
+Proof.
+  intros H contra.
+  apply f_equal with (f:=smt_to_verilog_var) in contra.
+  rewrite H in contra.
+  rewrite verilog_to_smt_to_verilog_var in contra.
+  discriminate.
+Qed.
+
 Import EqNotations.
 
-Definition execution_of_valuation (tag : TaggedVariable.Tag) (m : VerilogSMTBijection.t) (ρ : SMTLib.valuation) : execution :=
-  fun var =>
-    match m (tag, var) with
-    | Some smtName => XBV.from_bv (ρ (SMTLib.Sort_BitVec (Verilog.varType var)) smtName)
-    | None => XBV.exes _
-    end
-.
+Definition execution_of_valuation (tag : VarTag) (ρ : SMTLib.valuation) : execution :=
+  fun var => XBV.from_bv (ρ (verilog_to_smt_var tag var)).
 
-Lemma execution_of_valuation_defined_value tag (m : VerilogSMTBijection.t) ρ:
-  RegisterState.defined_value_for
-    (fun var => exists smtName, m (tag, var) = Some smtName)
-    (execution_of_valuation tag m ρ).
+Lemma execution_of_valuation_defined_value C tag ρ:
+  RegisterState.defined_value_for C (execution_of_valuation tag ρ).
 Proof.
   unfold execution_of_valuation.
-  intros var [smtName Hvar].
-  rewrite Hvar.
+  intros var _.
   eauto.
 Qed.
 
-Definition valuation_of_executions (m : VerilogSMTBijection.t) (e1 e2 : execution) : SMTLib.valuation :=
-  fun s smtName =>
-    match s as s' return SMTLib.interp_sort s' with
-    | SMTLib.Sort_Bool => default _
-    | SMTLib.Sort_BitVec w => 
-      match bij_inverse m smtName with
-| None => default _
-| Some (tag, verilogVar) =>
-  match dec (Verilog.varType verilogVar = w) with
-  | right _ => default _
-  | left E =>
-          let e :=
-            match tag with
-            | TaggedVariable.VerilogLeft => e1
-            | TaggedVariable.VerilogRight => e2
-            end
-          in
-            match XBV.to_bv (e verilogVar) with
-            (* TODO: Fix handling of Xs *)
-            | None => default _
-            | Some val => rew E in val
-            end
-  end
-end
-    end.
+Definition valuation_of_executions (e1 e2 : execution) : SMTLib.valuation :=
+  fun sym =>
+  match untag_name (SMTLib.symName sym), SMTLib.symSort sym with
+  | Some (t, varName), SMTLib.Sort_BitVec w =>
+    match dec (w > 0)%N with
+    | left prf =>
+      match XBV.to_bv (tag_choose t e1 e2 (Verilog.MkVariable varName w prf)) with
+      | Some bv => bv
+      | None => default (SMTLib.Sort_BitVec w)
+      end
+    | right _ => default (SMTLib.Sort_BitVec w)
+    end
+  | _, s => default s
+  end.
 
-Lemma execution_of_valuation_left_match_on (m : VerilogSMTBijection.t) e1 e2 l :
+Lemma execution_of_valuation_left_match_on e1 e2 l :
   RegisterState.defined_value_for (fun var => In var l) e1 ->
-  match_map_vars TaggedVariable.VerilogLeft m l ->
-  execution_of_valuation TaggedVariable.VerilogLeft m
-    (valuation_of_executions m e1 e2) =( l )= e1.
+  execution_of_valuation VerilogLeft
+    (valuation_of_executions e1 e2) =( l )= e1.
 Proof.
-  unfold execution_of_valuation, valuation_of_executions.
   (* intros Hdefined Hexists var Hvar_in. *)
-  intros Hdefined Hmatch var Hvar_in.
-  pose proof Hvar_in as H.
-  apply Hmatch in H. destruct H as [smtName HsmtName].
-  rewrite HsmtName.
-  rewrite VerilogSMTBijection.bij_wf in HsmtName.
-  rewrite HsmtName.
-  apply Hdefined in Hvar_in. destruct Hvar_in as [bv Hbv].
-  rewrite Hbv, XBV.xbv_bv_inverse.
-  autodestruct; [|contradiction].
-  rewrite <- eq_rect_eq.
-  reflexivity.
+  intros Hdefined var Hvar_in.
+  unfold valuation_of_executions, execution_of_valuation, verilog_to_smt_var.
+  destruct var. simpl.
+  destruct (dec (varType > 0)%N) as [varTypeWf'|?]; [|contradiction].
+  replace varTypeWf' with varTypeWf in * by apply proof_irrelevance.
+  autodestruct_eqn E.
+  - apply XBV.bv_xbv_inverse. assumption.
+  - exfalso.
+    edestruct Hdefined as [bv Hbv]; [apply Hvar_in|].
+    rewrite Hbv in E.
+    rewrite XBV.xbv_bv_inverse in E.
+    discriminate.
 Qed.
 
-Lemma execution_of_valuation_right_match_on (m : VerilogSMTBijection.t) e1 e2 l :
+Lemma execution_of_valuation_right_match_on e1 e2 l :
   RegisterState.defined_value_for (fun var => In var l) e2 ->
-  match_map_vars TaggedVariable.VerilogRight m l ->
-  execution_of_valuation TaggedVariable.VerilogRight m
-    (valuation_of_executions m e1 e2) =( l )= e2.
+  execution_of_valuation VerilogRight
+    (valuation_of_executions e1 e2) =( l )= e2.
 Proof.
-  unfold execution_of_valuation, valuation_of_executions.
   (* intros Hdefined Hexists var Hvar_in. *)
-  intros Hdefined Hmatch var Hvar_in.
-  pose proof Hvar_in as H.
-  apply Hmatch in H. destruct H as [smtName HsmtName].
-  rewrite HsmtName.
-  rewrite VerilogSMTBijection.bij_wf in HsmtName.
-  rewrite HsmtName.
-  apply Hdefined in Hvar_in. destruct Hvar_in as [bv Hbv].
-  rewrite Hbv, XBV.xbv_bv_inverse.
-  autodestruct; [|contradiction].
-  rewrite <- eq_rect_eq.
-  reflexivity.
+  intros Hdefined var Hvar_in.
+  unfold valuation_of_executions, execution_of_valuation, verilog_to_smt_var.
+  destruct var. simpl.
+  destruct (dec (varType > 0)%N) as [varTypeWf'|?]; [|contradiction].
+  replace varTypeWf' with varTypeWf in * by apply proof_irrelevance.
+  autodestruct_eqn E.
+  - apply XBV.bv_xbv_inverse. assumption.
+  - exfalso.
+    edestruct Hdefined as [bv Hbv]; [apply Hvar_in|].
+    rewrite Hbv in E.
+    rewrite XBV.xbv_bv_inverse in E.
+    discriminate.
 Qed.
 
-Definition verilog_smt_match_on_name (regs : RegisterState.t) (ρ : SMTLib.valuation) var smtName : Prop :=
-  regs var = XBV.from_bv (ρ (SMTLib.Sort_BitVec (Verilog.varType var)) smtName).
-    
 Definition verilog_smt_match_states_partial
   (cond : Verilog.variable -> Prop)
-  (tag : TaggedVariable.Tag)
-  (m : VerilogSMTBijection.t)
+  (tag : VarTag)
   (regs : RegisterState.t)
   (ρ : SMTLib.valuation) : Prop :=
-  forall var,
-    cond var ->
-    exists smtName,
-      m (tag, var) = Some smtName
-      /\ verilog_smt_match_on_name regs ρ var smtName.
+  forall var, cond var -> regs var = XBV.from_bv (ρ (verilog_to_smt_var tag var)).
 
 (* Might not be needed *)
 Global Instance verilog_smt_match_states_partial_proper :
   Proper
-    (pointwise_relation Verilog.variable iff ==> eq ==> eq ==> eq ==> eq ==> iff)
+    (pointwise_relation Verilog.variable iff ==> eq ==> eq ==> eq ==> iff)
     verilog_smt_match_states_partial.
 Proof.
   repeat intro. subst.
@@ -251,59 +240,47 @@ Qed.
 
 Global Instance verilog_smt_match_states_partial_impl_proper :
   Proper
-    (pointwise_relation Verilog.variable Basics.impl ==> eq ==> eq ==> eq ==> eq ==> Basics.flip Basics.impl)
+    (pointwise_relation Verilog.variable Basics.impl ==> eq ==> eq ==> eq ==> Basics.flip Basics.impl)
     verilog_smt_match_states_partial.
 Proof.
   repeat intro. subst.
   crush.
 Qed.
 
-Lemma verilog_smt_match_states_execution_of_valuation_same tag (m : VerilogSMTBijection.t) ρ :
-  verilog_smt_match_states_partial (fun var => exists smtName, m (tag, var) = Some smtName) tag m (execution_of_valuation tag m ρ) ρ.
+Lemma verilog_smt_match_states_execution_of_valuation_same C tag ρ :
+  verilog_smt_match_states_partial C tag (execution_of_valuation tag ρ) ρ.
 Proof.
   intros Hhas_var.
   unfold verilog_smt_match_states_partial, execution_of_valuation.
-  intros [smtName HsmtName].
-  exists smtName. split; [eassumption|].
-  unfold verilog_smt_match_on_name.
-  rewrite HsmtName.
-  reflexivity.
+  crush.
 Qed.
 
-Lemma verilog_smt_match_states_partial_impl P1 P2 tag m regs ρ :
+Lemma verilog_smt_match_states_partial_impl P1 P2 tag regs ρ :
   (forall x, P2 x -> P1 x) ->
-  verilog_smt_match_states_partial P1 tag m regs ρ ->
-  verilog_smt_match_states_partial P2 tag m regs ρ.
+  verilog_smt_match_states_partial P1 tag regs ρ ->
+  verilog_smt_match_states_partial P2 tag regs ρ.
 Proof. crush. Qed.
 
-Lemma verilog_smt_match_states_partial_set_reg_out C tag m r ρ var val :
+Lemma verilog_smt_match_states_partial_set_reg_out C tag r ρ var val :
   ~ C var ->
-  verilog_smt_match_states_partial C tag m (RegisterState.set_reg var val r) ρ <->
-  verilog_smt_match_states_partial C tag m r ρ.
+  verilog_smt_match_states_partial C tag (RegisterState.set_reg var val r) ρ <->
+  verilog_smt_match_states_partial C tag r ρ.
 Proof.
   intro Hcond1.
   unfold verilog_smt_match_states_partial.
-  unfold verilog_smt_match_on_name in *.
-  split; intros H * Hcond2.
-  - destruct (dec (var0 = var)).
-    + subst. contradiction.
-    + insterU H. destruct H as [smtName [? Hverilogval]].
-      econstructor. split. { eassumption. }
-      rewrite RegisterState.set_reg_get_out in Hverilogval by congruence.
-      assumption.
-  - destruct (dec (var0 = var)).
-    + subst. contradiction.
-    + insterU H. destruct H as [smtName [? Hverilogval]].
-      econstructor. split. { eassumption. }
-      rewrite RegisterState.set_reg_get_out by congruence.
-      assumption.
+  split.
+  all: intros H * Hcond2.
+  all: destruct (dec (var0 = var)); [subst; contradiction|].
+  all: rewrite <- H by assumption.
+  all: rewrite RegisterState.set_reg_get_out by congruence.
+  all: reflexivity.
 Qed.
 
-Lemma verilog_smt_match_states_partial_split C1 C2 C3 tag m reg ρ :
+Lemma verilog_smt_match_states_partial_split C1 C2 C3 tag reg ρ :
   (forall var, C3 var -> C1 var \/ C2 var) ->
-  verilog_smt_match_states_partial C1 tag m reg ρ ->
-  verilog_smt_match_states_partial C2 tag m reg ρ ->
-  verilog_smt_match_states_partial C3 tag m reg ρ.
+  verilog_smt_match_states_partial C1 tag reg ρ ->
+  verilog_smt_match_states_partial C2 tag reg ρ ->
+  verilog_smt_match_states_partial C3 tag reg ρ.
 Proof.
   unfold verilog_smt_match_states_partial.
   intros Himpl H1 H2 * HC3.
@@ -311,146 +288,91 @@ Proof.
   destruct HC3; eauto.
 Qed.
 
-Lemma verilog_smt_match_states_partial_split_iff C1 C2 tag m reg ρ :
-  verilog_smt_match_states_partial (fun var => C1 var \/ C2 var) tag m reg ρ <->
-    (verilog_smt_match_states_partial C1 tag m reg ρ
-     /\ verilog_smt_match_states_partial C2 tag m reg ρ).
+Lemma verilog_smt_match_states_partial_split_iff C1 C2 tag reg ρ :
+  verilog_smt_match_states_partial (fun var => C1 var \/ C2 var) tag reg ρ <->
+    (verilog_smt_match_states_partial C1 tag reg ρ
+     /\ verilog_smt_match_states_partial C2 tag reg ρ).
 Proof. unfold verilog_smt_match_states_partial. crush. Qed.
 
-Lemma verilog_smt_match_states_partial_set_reg_elim C tag (m : VerilogSMTBijection.t) regs ρ var bv :
-  (exists smtName,
-      m (tag, var) = Some smtName /\ ρ (SMTLib.Sort_BitVec (Verilog.varType var)) smtName = bv) ->
-  verilog_smt_match_states_partial C tag m regs ρ ->
-  verilog_smt_match_states_partial C tag m (RegisterState.set_reg var (XBV.from_bv bv) regs) ρ.
+Lemma verilog_smt_match_states_partial_set_reg_elim C tag regs ρ var bv :
+  (ρ (verilog_to_smt_var tag var) = bv) ->
+  verilog_smt_match_states_partial C tag regs ρ ->
+  verilog_smt_match_states_partial C tag (RegisterState.set_reg var (XBV.from_bv bv) regs) ρ.
 Proof.
   unfold verilog_smt_match_states_partial.
-  unfold verilog_smt_match_on_name.
   intros Hvar Hrest *.
   destruct (dec (var0 = var)); intros Hcond.
   - subst.
-    insterU Hvar. destruct Hvar as [? [? ?]].
-    insterU Hrest. destruct Hrest as [? [? ?]].
-    replace x0 with x in * by congruence.
-    repeat econstructor; try eassumption; expect 1.
-    rewrite RegisterState.set_reg_get_in.
-    repeat f_equal.
-    congruence.
-  - insterU Hvar. destruct Hvar as [? [? ?]].
-    insterU Hrest. destruct Hrest as [? [? ?]].
-    repeat econstructor; try eassumption; expect 1.
-    rewrite RegisterState.set_reg_get_out; eauto.
+    apply RegisterState.set_reg_get_in.
+  - rewrite RegisterState.set_reg_get_out by congruence.
+    apply Hrest. apply Hcond.
 Qed.
 
-Lemma verilog_smt_match_states_partial_change_regs C tag m r1 r2 ρ :
+Lemma verilog_smt_match_states_partial_change_regs C tag r1 r2 ρ :
   (forall var, C var -> r1 var = r2 var) ->
-  verilog_smt_match_states_partial C tag m r1 ρ ->
-  verilog_smt_match_states_partial C tag m r2 ρ.
+  verilog_smt_match_states_partial C tag r1 ρ ->
+  verilog_smt_match_states_partial C tag r2 ρ.
 Proof.
   unfold verilog_smt_match_states_partial.
   intros Hsame Hmatch1 * Hcond.
   insterU Hsame. insterU Hcond. insterU Hmatch1.
-  destruct Hmatch1 as [smtName [? ?]].
-  exists smtName.
-  split. { eassumption. }
-  unfold verilog_smt_match_on_name in *.
   congruence.
 Qed.
 
 Ltac unpack_verilog_smt_match_states_partial :=
   repeat match goal with
-    | [ H: verilog_smt_match_states_partial (fun _ => _ \/ _) _ _ _ _ |- _ ] =>
+    | [ H: verilog_smt_match_states_partial (fun _ => _ \/ _) _ _ _ |- _ ] =>
         apply verilog_smt_match_states_partial_split_iff in H;
         destruct H
-    | [ H: verilog_smt_match_states_partial (fun _ => List.In _ (_ ++ _)) _ _ _ _ |- _ ] =>
+    | [ H: verilog_smt_match_states_partial (fun _ => List.In _ (_ ++ _)) _ _ _ |- _ ] =>
         setoid_rewrite List.in_app_iff in H
-    | [ |- verilog_smt_match_states_partial (fun _ => List.In _ (_ ++ _)) _ _ _ _ ] =>
+    | [ |- verilog_smt_match_states_partial (fun _ => List.In _ (_ ++ _)) _ _ _ ] =>
         setoid_rewrite List.in_app_iff
-    | [ |- verilog_smt_match_states_partial (fun _ => _ \/ _) _ _ _ _ ] =>
+    | [ |- verilog_smt_match_states_partial (fun _ => _ \/ _) _ _ _ ] =>
         apply verilog_smt_match_states_partial_split_iff; split
     end.
 
-Lemma verilog_smt_match_states_partial_defined_value_for C tag m regs ρ :
-  verilog_smt_match_states_partial C tag m regs ρ ->
+Lemma verilog_smt_match_states_partial_defined_value_for C tag regs ρ :
+  verilog_smt_match_states_partial C tag regs ρ ->
   RegisterState.defined_value_for C regs.
 Proof.
-  unfold verilog_smt_match_states_partial, verilog_smt_match_on_name, RegisterState.defined_value_for.
+  unfold verilog_smt_match_states_partial, RegisterState.defined_value_for.
   intros Hmatch * Hcond.
-  edestruct Hmatch as [? [? ?]]; eauto.
+  eauto.
 Qed.
 
-Lemma verilog_smt_match_states_partial_execution_match_on C tag m ρ e :
-    verilog_smt_match_states_partial C tag m e ρ ->
-    e ={ C }= execution_of_valuation tag m ρ.
+Lemma verilog_smt_match_states_partial_execution_match_on C tag ρ e :
+    verilog_smt_match_states_partial C tag e ρ ->
+    e ={ C }= execution_of_valuation tag ρ.
 Proof.
   unfold verilog_smt_match_states_partial, "_ ={ _ }= _".
-  unfold verilog_smt_match_on_name.
   intros H var Hvar.
-  edestruct H as [? [H1 H2]]; [eauto|].
-  unfold execution_of_valuation.
-  rewrite H1. assumption.
+  apply H.
+  apply Hvar.
 Qed.
 
-Lemma verilog_smt_match_states_partial_execution_defined_value_for C tag m ρ e :
-    verilog_smt_match_states_partial C tag m e ρ ->
+Lemma verilog_smt_match_states_partial_execution_defined_value_for C tag ρ e :
+    verilog_smt_match_states_partial C tag e ρ ->
     RegisterState.defined_value_for C e.
 Proof.
   unfold verilog_smt_match_states_partial, RegisterState.defined_value_for.
   intros H var Hvar.
-  edestruct H as [? [H1 H2]]; [eauto|].
-  inv H2. eauto.
+  rewrite H by assumption.
+  eauto.
 Qed.
 
-Lemma execution_of_valuation_inv tag m ρ var bv :
-  execution_of_valuation tag m ρ var = XBV.from_bv bv ->
-  exists smtName,
-    m (tag, var) = Some smtName /\
-    ρ (SMTLib.Sort_BitVec (Verilog.varType var)) smtName = bv .
+Lemma execution_of_valuation_inv tag ρ var bv :
+  execution_of_valuation tag ρ var = XBV.from_bv bv ->
+  ρ (verilog_to_smt_var tag var) = bv.
 Proof.
   unfold execution_of_valuation.
-  intros H.
-  (* We don't know that var is in m. We could have added it directly
-  as an assumption, but we can also deduce it from the fact that the
-  value of the var in e is defined. This is only possible, however, if
-  the var is not zero-width (because zero-width Xs are
-  indistinguishable from zero-width 0/1s). This lemma is why we have
-  added varTypeWf into verilog variables *)
-
-  destruct (m (tag, var)).
-  - apply XBV.from_bv_injective in H.
-    eauto.
-  - exfalso.
-    apply f_equal with (f:=XBV.to_bv) in H.
-    autorewrite with xbv in H.
-    rewrite XBV.exes_to_bv in H by apply Verilog.varTypeWf.
-    discriminate.
+  apply XBV.from_bv_injective.
 Qed.
 
-Lemma execution_match_on_verilog_smt_match_states_partial C tag m ρ e :
-    RegisterState.defined_value_for C e ->
-    e ={ C }= (execution_of_valuation tag m ρ) ->
-    verilog_smt_match_states_partial C tag m e ρ.
+Lemma execution_match_on_verilog_smt_match_states_partial C tag ρ e :
+    e ={ C }= (execution_of_valuation tag ρ) ->
+    verilog_smt_match_states_partial C tag e ρ.
 Proof.
-  unfold RegisterState.defined_value_for, verilog_smt_match_states_partial, "_ =( _ )= _".
-  intros Hdefined Heq var Hvar.
-  insterU Hdefined. insterU Heq.
-  destruct Hdefined as [bv Hbv]. 
-  unfold verilog_smt_match_on_name in *.
-  unfold execution_of_valuation in *.
-
-  (* TODO: Use execution_of_valuation_inv instead. *)
-
-  (* We don't know that var is in m. We could have added it directly
-  as an assumption, but we can also deduce it from the fact that the
-  value of the var in e is defined. This is only possible, however, if
-  the var is not zero-width (because zero-width Xs are
-  indistinguishable from zero-width 0/1s). This lemma is why we have
-  added varTypeWf into verilog variables *)
-
-  destruct (m (tag, var)); [solve [eauto]|].
-  exfalso.
-  rewrite Hbv in Heq. clear Hbv.
-  apply f_equal with (f:=XBV.to_bv) in Heq.
-  autorewrite with xbv in Heq.
-  rewrite XBV.exes_to_bv in Heq by apply Verilog.varTypeWf.
-  discriminate.
+  unfold execution_of_valuation, verilog_smt_match_states_partial, "_ =( _ )= _".
+  trivial.
 Qed.
